from 60s to 39s using compression of reals (underlying rationals).
It was implemented in CoRN.reals.fast.Compress, and used in
CoRN.reals.faster.ARQ

Also generalized the SinClass to make it possible to reuse the same code
for specialized implementations of sine where the domain is different
from the codomain: e.g. rational_sin : Q -> CR.

src/fastReals/interface.v
@@ -28,8 +28,13 @@
 
 Class MinClass (A:Type) := min : A -> A -> A.
 Class MaxClass (A:Type) := max : A -> A -> A.
-Class SinClass (A:Type) := sin : A -> A.
-Class CosClass (A:Type) := cos : A -> A.
+
+(** generalized Sin Class. The domain may be some kind of (approx) rationals *)
+Class GSinClass (B  A : Type) := gsin :  B->A.
+Class GCosClass (B  A : Type) := gcos :  B->A.
+
+Class SinClass (A:Type) := sin :> GSinClass A A.
+Class CosClass (A:Type) := cos :> GCosClass A A.
 
 Require Import ROSCOQ.IRMisc.CoRNMisc.
 (**because most of the theory of analysis in CoRN is built for IR. These might
